ironfleet/src/Dafny/Distributed/Protocol/RSL/FailureProof/Phase1/GenericLemmas.i.dfy
@@ -126,4 +126,144 @@ lemma lemma_NonLeaderDoesNotSend1a_Undelivered(ts:TimestampedRslState, ts':Times
     }
 }
 
+
+/* There can be no 2b messages sent in a Non-Receive step  */
+lemma lemma_No2bSentInNonReceiveStep(ts:TimestampedRslState, ts':TimestampedRslState, op:OperationNumber, idx:int, tios:seq<TimestampedLIoOp<NodeIdentity, RslMessage>>) 
+    requires CommonAssumptions(ts) && CommonAssumptions(ts')
+    requires P1Assumption(ts, op)
+    requires TimestampedRslNext(ts, ts')
+    requires !TimestampedRslNextEnvironment(ts, ts')
+    requires TimestampedRslNextOneReplica(ts, ts', idx, tios)
+    requires Phase1Invariant(ts, op)
+    requires idx != 0
+    requires ts.t_replicas[idx].v.nextActionIndex != 0
+    ensures forall pkt | pkt in ts'.t_environment.sentPackets && pkt.msg.v.RslMessage_2b? :: pkt in ts.t_environment.sentPackets
+    ensures forall pkt | pkt in ts'.undeliveredPackets && pkt.msg.v.RslMessage_2b? :: pkt in ts.undeliveredPackets
+{
+    assume false;
+    // var ls, ls' := ts.t_replicas[idx], ts'.t_replicas[idx];
+    // var nextActionIndex := ls.v.nextActionIndex;
+    // forall pkt | pkt in ts'.t_environment.sentPackets && pkt.msg.v.RslMessage_2b?
+    // ensures pkt in ts.t_environment.sentPackets 
+    // {
+    //     if pkt !in ts.t_environment.sentPackets {
+    //         var ios := UntagLIoOpSeq(tios);
+    //         var sent_packets := ExtractSentPacketsFromIos(ios);
+    //         assert LReplicaNoReceiveNext(ls.v.replica, nextActionIndex, ls'.v.replica, ios);
+    //         assert forall p | p in sent_packets :: !p.msg.RslMessage_2b?;
+    //         forall io | io in tios && io.LIoOpSend?
+    //         ensures !io.s.msg.v.RslMessage_2b? {}
+    //         assert false;
+    //     }
+    // }
+    // lemma_No2bSentInNonReceiveStep_Undelivered(ts, ts', op, idx, tios);
+}
+
+
+lemma lemma_No2bSentInNonReceiveStep_Undelivered(ts:TimestampedRslState, ts':TimestampedRslState, op:OperationNumber, idx:int, tios:seq<TimestampedLIoOp<NodeIdentity, RslMessage>>) 
+    requires CommonAssumptions(ts) && CommonAssumptions(ts')
+    requires P1Assumption(ts, op)
+    requires TimestampedRslNext(ts, ts')
+    requires !TimestampedRslNextEnvironment(ts, ts')
+    requires TimestampedRslNextOneReplica(ts, ts', idx, tios)
+    requires Phase1Invariant(ts, op)
+    requires idx != 0
+    requires ts.t_replicas[idx].v.nextActionIndex != 0
+    ensures forall pkt | pkt in ts'.undeliveredPackets && pkt.msg.v.RslMessage_2b? :: pkt in ts.undeliveredPackets
+{
+    assume false;
+    // var ls, ls' := ts.t_replicas[idx], ts'.t_replicas[idx];
+    // var nextActionIndex := ls.v.nextActionIndex;
+    // forall pkt | pkt in ts'.undeliveredPackets && pkt.msg.v.RslMessage_2b?
+    // ensures pkt in ts.undeliveredPackets
+    // {
+    //     if pkt !in ts.undeliveredPackets {
+    //         var ios := UntagLIoOpSeq(tios);
+    //         var sent_packets := ExtractSentPacketsFromIos(ios);
+    //         assert LReplicaNoReceiveNext(ls.v.replica, nextActionIndex, ls'.v.replica, ios);
+    //         assert forall p | p in sent_packets :: !p.msg.RslMessage_2b?;
+    //         forall io | io in tios && io.LIoOpSend?
+    //         ensures !io.s.msg.v.RslMessage_2b? {}
+    //         assert false;
+    //     }
+    // }
+}
+
+
+lemma lemma_No1bSentInNonReceiveStep(ts:TimestampedRslState, ts':TimestampedRslState, op:OperationNumber, idx:int, tios:seq<TimestampedLIoOp<NodeIdentity, RslMessage>>) 
+    requires CommonAssumptions(ts) && CommonAssumptions(ts')
+    requires P1Assumption(ts, op)
+    requires TimestampedRslNext(ts, ts')
+    requires !TimestampedRslNextEnvironment(ts, ts')
+    requires TimestampedRslNextOneReplica(ts, ts', idx, tios)
+    requires Phase1Invariant(ts, op)
+    requires idx != 0
+    requires ts.t_replicas[idx].v.nextActionIndex != 0
+    ensures forall pkt | pkt in ts'.t_environment.sentPackets && pkt.msg.v.RslMessage_1b? :: pkt in ts.t_environment.sentPackets
+    ensures forall pkt | pkt in ts'.undeliveredPackets && pkt.msg.v.RslMessage_1b? :: pkt in ts.undeliveredPackets
+{
+    //TODO
+    assume false;
+}
+
+
+/* There can be no 2a messages sent in a non-NominateValueAndSend2a step  */
+lemma {:timeLimitMultiplier 2} lemma_No2aSentInNon2aStep(ts:TimestampedRslState, ts':TimestampedRslState, op:OperationNumber, idx:int, tios:seq<TimestampedLIoOp<NodeIdentity, RslMessage>>) 
+    requires CommonAssumptions(ts) && CommonAssumptions(ts')
+    requires P1Assumption(ts, op)
+    requires TimestampedRslNext(ts, ts')
+    requires !TimestampedRslNextEnvironment(ts, ts')
+    requires TimestampedRslNextOneReplica(ts, ts', idx, tios)
+    requires Phase1Invariant(ts, op)
+    requires idx != 0
+    requires ts.t_replicas[idx].v.nextActionIndex != 3
+    ensures forall pkt | pkt in ts'.t_environment.sentPackets && pkt.msg.v.RslMessage_2a? :: pkt in ts.t_environment.sentPackets
+    ensures forall p | p in ts'.undeliveredPackets && p.msg.v.RslMessage_2a? :: p in ts.undeliveredPackets
+{
+    assume false;
+    // var ls, ls' := ts.t_replicas[idx], ts'.t_replicas[idx];
+    // var nextActionIndex := ls.v.nextActionIndex;
+
+    // forall p | p in ts'.t_environment.sentPackets && p.msg.v.RslMessage_2a?
+    // ensures p in ts.t_environment.sentPackets {
+    //     if p !in ts.t_environment.sentPackets {
+    //         if nextActionIndex == 3 {
+    //             assert false;
+    //         } else {
+    //             forall io | io in tios && io.LIoOpSend?
+    //             ensures !io.s.msg.v.RslMessage_2a? {}
+    //             assert false;
+    //         }
+    //     }
+    // }
+    // forall p | p in ts'.undeliveredPackets && p.msg.v.RslMessage_2a?
+    // ensures p in ts.undeliveredPackets {
+    //     if p !in ts.undeliveredPackets {
+    //         if nextActionIndex == 3 {
+    //             assert false;
+    //         } else {
+    //             forall io | io in tios && io.LIoOpSend?
+    //             ensures !io.s.msg.v.RslMessage_2a? {}
+    //             assert false;
+    //         }
+    //     }
+    // }
+}
+
+
+/* There can be no Reply messages sent in a Non-Execution step  */
+lemma lemma_NoRepliesSentInNonExecutionStep(ts:TimestampedRslState, ts':TimestampedRslState, op:OperationNumber, idx:int, tios:seq<TimestampedLIoOp<NodeIdentity, RslMessage>>) 
+    requires CommonAssumptions(ts) && CommonAssumptions(ts')
+    requires P1Assumption(ts, op)
+    requires TimestampedRslNext(ts, ts')
+    requires !TimestampedRslNextEnvironment(ts, ts')
+    requires TimestampedRslNextOneReplica(ts, ts', idx, tios)
+    requires Phase1Invariant(ts, op)
+    requires idx != 0
+    requires ts.t_replicas[idx].v.nextActionIndex != 6
+    ensures forall pkt | pkt in ts'.t_environment.sentPackets && IsNewReplyPacket(ts', pkt) :: pkt in ts.t_environment.sentPackets
+{
+    assume false;
+}
+
 }
