ironfleet/src/Dafny/Distributed/Protocol/RSL/FailureProof/Phase1/Phase1Proof_helper2.i.dfy
@@ -1,0 +1,128 @@
+include "Phase1Proof.i.dfy"
+include "GenericLemmas.i.dfy"
+
+module RslPhase1Proof_Helper2 {
+import opened RslPhase1Proof_i
+import opened RslPhase1Proof_Generic
+
+
+/* Proof that a Phase1 state maybe transitions to a Phase2 state when nextAction == 2 */
+lemma Phase1_to_MaybePhase2(ts:TimestampedRslState, ts':TimestampedRslState, opn:OperationNumber, idx:int, tios:seq<TimestampedLIoOp<NodeIdentity, RslMessage>>) 
+    requires CommonAssumptions(ts) && CommonAssumptions(ts')
+    requires P1Assumption(ts, opn)
+    requires InPhase1(ts') ==> P1Assumption(ts', opn)
+    requires TimestampedRslNext(ts, ts')
+    requires Phase1Invariant(ts, opn)
+    requires TimestampedRslNextOneReplica(ts, ts', idx, tios);
+    requires ts.t_replicas[idx].v.nextActionIndex == 2
+    requires idx != 0
+    ensures InPhase1(ts') || InPhase2(ts')
+    ensures InPhase1(ts') ==> Phase1Invariant(ts', opn)
+    ensures InPhase2(ts') ==> P2.Phase2Invariant(ts', opn)
+{
+    if idx == 1 {
+        var ls, ls' := ts.t_replicas[idx], ts'.t_replicas[idx];
+        var goToPhase2 :=  && |ls.v.replica.proposer.received_1b_packets| >= LMinQuorumSize(ls.v.replica.proposer.constants.all.config)
+                           && LSetOfMessage1bAboutBallot(ls.v.replica.proposer.received_1b_packets, ls.v.replica.proposer.max_ballot_i_sent_1a);
+        if goToPhase2 {
+            Phase1_to_Phase2(ts, ts', opn, tios);
+        } else {
+            // TODO
+            assume false;
+        }
+    } else {
+        assert InPhase1(ts');
+        assert Phase1Invariant(ts', opn);
+    }
+}
+
+
+lemma Phase1_to_Phase2(ts:TimestampedRslState, ts':TimestampedRslState, opn:OperationNumber, tios:seq<TimestampedLIoOp<NodeIdentity, RslMessage>>) 
+    requires CommonAssumptions(ts) && CommonAssumptions(ts')
+    requires P1Assumption(ts, opn)
+    requires InPhase1(ts') ==> P1Assumption(ts', opn)
+    requires TimestampedRslNext(ts, ts')
+    requires Phase1Invariant(ts, opn)
+    requires TimestampedRslNextOneReplica(ts, ts', 1, tios);
+    requires ts.t_replicas[1].v.nextActionIndex == 2
+    requires && |ts.t_replicas[1].v.replica.proposer.received_1b_packets| >= LMinQuorumSize(ts.t_replicas[1].v.replica.proposer.constants.all.config)
+             && LSetOfMessage1bAboutBallot(ts.t_replicas[1].v.replica.proposer.received_1b_packets, ts.t_replicas[1].v.replica.proposer.max_ballot_i_sent_1a);
+    ensures InPhase2(ts')
+    ensures P2.Phase2Invariant(ts', opn)
+{
+    var ls, ls' := ts.t_replicas[1], ts'.t_replicas[1];
+    assert InPhase2(ts');
+
+    lemma_No2aSentInNon2aStep(ts, ts', opn, 1, tios);
+    lemma_No2bSentInNonReceiveStep(ts, ts', opn, 1, tios);
+    lemma_NoRepliesSentInNonExecutionStep(ts, ts', opn, 1, tios);
+    Phase1_to_Phase2_RequestSrcAndBatchSize(ts, ts', opn, tios);
+
+    assert TimeLe(ls'.ts, TimeBoundPhase1LeaderPost(3));
+    assert TimeLe(ls'.ts, NewLeaderP2_InitTS); 
+    assert P2.Before_2a_Sent_Invariant(ts', opn);
+}
+
+
+lemma Phase1_to_Phase2_RequestSrcAndBatchSize(ts:TimestampedRslState, ts':TimestampedRslState, opn:OperationNumber, tios:seq<TimestampedLIoOp<NodeIdentity, RslMessage>>) 
+    requires CommonAssumptions(ts) && CommonAssumptions(ts')
+    requires P1Assumption(ts, opn)
+    requires InPhase1(ts') ==> P1Assumption(ts', opn)
+    requires TimestampedRslNext(ts, ts')
+    requires Phase1Invariant(ts, opn)
+    requires TimestampedRslNextOneReplica(ts, ts', 1, tios);
+    requires ts.t_replicas[1].v.nextActionIndex == 2
+    requires InPhase2(ts')
+    requires P2.AlwaysInvariantP2_RequestSrcAndBatchSize(ts, opn)
+    ensures P2.AlwaysInvariantP2_RequestSrcAndBatchSize(ts', opn)
+{
+    var ls, ls' := ts.t_replicas[1], ts'.t_replicas[1];
+
+    // RequestSrcAndBatchSize -- 1b
+    forall p, op| IsUndelivered_1bPkt(ts', p) && op in p.msg.v.votes   
+    ensures && RequestBatchSrcInClientIds(ts', p.msg.v.votes[op].max_val)
+            && |p.msg.v.votes[op].max_val| > 0
+    {
+        lemma_No1bSentInNonReceiveStep(ts, ts', opn, 1, tios);
+        assert IsUndelivered_1bPkt(ts, p);
+        forall r | r in p.msg.v.votes[op].max_val
+        ensures r.client in ts'.constants.config.clientIds {}
+    }
+
+    // RequestSrcAndBatchSize -- 2a
+    forall p | IsUndelivered_2aPkt(ts', p)   
+    ensures && RequestBatchSrcInClientIds(ts', p.msg.v.val_2a)
+            && |p.msg.v.val_2a| > 0
+    {
+        lemma_No2aSentInNon2aStep(ts, ts', opn, 1, tios);
+        assert IsUndelivered_2aPkt(ts, p);
+        forall r | r in p.msg.v.val_2a
+        ensures r.client in ts'.constants.config.clientIds
+        {}
+    }
+
+    // RequestSrcAndBatchSize -- 2b
+    lemma_No2bSentInNonReceiveStep(ts, ts', opn, 1, tios);
+
+    // RequestSrcAndBatchSize -- leader's received_1b_packets set
+    forall p, op | p in ls'.v.replica.proposer.received_1b_packets && p.msg.RslMessage_1b? && op in p.msg.votes
+    ensures RequestBatchSrcInClientIds(ts', p.msg.votes[op].max_val)
+    {
+        assert p in ls.v.replica.proposer.received_1b_packets;
+        forall r | r in p.msg.votes[op].max_val
+        ensures r.client in ts'.constants.config.clientIds {}
+    }
+
+    // RequestSrcAndBatchSize -- Acceptors
+    forall i, op| 0 <= i < |ts'.t_replicas| && op in ts'.t_replicas[i].v.replica.acceptor.votes
+    ensures && |ts'.t_replicas[i].v.replica.acceptor.votes[op].max_val| > 0   
+            &&  RequestBatchSrcInClientIds(ts', ts'.t_replicas[i].v.replica.acceptor.votes[op].max_val)
+    {
+        assert ls'.v.replica.acceptor == ls.v.replica.acceptor;
+        forall r | r in ts'.t_replicas[i].v.replica.acceptor.votes[op].max_val
+        ensures r.client in ts'.constants.config.clientIds {}
+    }   
+}
+
+
+}
